Multiple fixes to the definability which do not break the previous spec
Furthurmore, it helped getting rid of the NOP hack (which broke the
specs). Mainly, the changes consist in the use of pmap instead of map in
expr_of_trace, expr_of_event returns an option : no need to return dummy
expressions, only events triggered by the component return expressions.

The proof of well_formed_events_well_formed_program is fixed wrt this,
the counter value is defined by only the number of events triggered by a
component C, proofs up to 'definability_gen' are fixed and so is the
base case of the latter.

Source/Definability.v
@@ -95,21 +95,16 @@ Section Definability.
    *)
 
   Definition counter_idx : Block.offset := 0%Z.
+  Definition counter_loc : expr := E_local Block.priv.
   Definition increment exp_val := E_binop Add exp_val (E_val (Int 1%Z)).
 
-  Definition FAIL : expr := E_val Undef.
-  (* Maybe define NOP in language in order to avoir such a workaround (or use
-     another expression).
-     Should be fine since this would just set R_COM to 0, and R_COM would be
-     redefined before used *)
-  Definition NOP : expr := E_val (Int 0).
-
-  Hint Unfold increment counter_idx NOP.
+  Hint Unfold increment counter_idx counter_loc.
+  Hint Transparent increment counter_idx counter_loc.
 
   Definition switch_clause n e_then e_else :=
     E_if (E_binop Eq (E_deref (E_local Block.priv)) (E_val (Int n)))
          (E_seq (E_assign (E_local Block.priv)
-                          (increment (E_deref (E_local Block.priv)))) e_then)
+                          (increment (E_deref counter_loc))) e_then)
          e_else.
 
   Ltac take_step :=
@@ -458,12 +453,14 @@ Section Definability.
   (* I find that checking fmap membership, even for map with given static data,
      is a bit of a pain. It would be nice to add these to the 'done' tactical or
      some other automation mean *)
-  Example setm_thingy :
+  Example setm_fmap_membership :
     let fmap_thing := [fmap (0, false); (1, false); (2, false)] in
     let fset_thing := [fset 0; 1; 2] in
      1 \in domm fmap_thing /\ false \in codomm fmap_thing /\ 1 \in fset_thing.
   Proof.
     simpl. split.
+    (* Not automated yet *)
+    all: simpl; try done.
     (* \in domm of something is usually solved automatically once mem_domm has
          been used *)
     rewrite mem_domm ; done. Undo.
@@ -677,7 +674,8 @@ Section Definability.
 
   Lemma prefill_read_aux_invar : forall suffix C comp acc indexes res ,
       intf C = Some comp ->
-      (* Add a restriction on the indexes wrt comp.public_buffer_size *)
+      (* Add a restriction on the indexes wrt comp.public_buffer_size ? case
+         analysis on indexes_read_init comp should suffice *)
       prefill_read_aux C suffix acc indexes (* (indexes_read_init comp) *) = res ->
       exists res', prefill_read_aux_ntr C suffix indexes = res' /\
               res = rev res' ++ acc.
@@ -819,9 +817,7 @@ Section Definability.
 
 
   (** Gives Some expr that is the (sequence of) assignement(s) or None if it's
-      not the case.
-      As said above, we can use rev' before flattening the list of expressions
-      to keep this tail-recursive *)
+      not the case. *)
   Definition prefill_read (C: Component.id) (suffix: trace) : option expr :=
     (* Only used to accomodate with the fact that the interface is a map.
        None is never returned by this match, but can be returned by
@@ -924,38 +920,34 @@ Section Definability.
       In the case we give turn to the component we're recreating (if it is
       called/ returned to), goes forward in the trace to make sure the
       subsequent ELoad would be successful. *)
-  Definition expr_of_event (C: Component.id) (P: Procedure.id) (suffix: trace) : expr :=
+  Definition expr_of_event (C: Component.id) (P: Procedure.id) (suffix: trace) : option expr :=
     match suffix with
-    (* Never happens except for an empty trace *)
-    | nil => NOP
+    | nil => None
     | ECall _ P' arg C' :: suffix' =>
       let call_trigger := E_seq (E_call C' P' (E_val (Int arg)))
                                 (E_call C  P  (E_val (Int 0))) in
       match (prefill_read C suffix') with
-      | None => call_trigger
-      | Some prefill => E_seq prefill call_trigger
+      | None => Some call_trigger
+      | Some prefill => Some (E_seq prefill call_trigger)
       end
     | ERet _ ret_val _ :: suffix' =>
       let return_trigger := E_val (Int ret_val) in
       match prefill_read C suffix' with
-      | None => return_trigger
-      | Some prefill => E_seq prefill return_trigger
+      | None => Some return_trigger
+      | Some prefill => Some (E_seq prefill return_trigger)
       end
     | ELoad C' off _ C'' :: suffix' =>
       (* In case of load performed by the current component *)
-      if C == C' then E_seq (E_deref (E_binop Add (E_component_buf C'') (E_val (Int off))))
-                            (E_assign (E_local Block.priv)
-                                      (increment (E_deref (E_local Block.priv))))
+      if C == C' then
+        Some (E_deref (E_binop Add (E_component_buf C'') (E_val (Int off))))
       else
         (* In the case the memory from the current component is loaded, we don't
            do anything here (this kind of event is used in prefill_read) *)
-        (* problem(?) : should produce nothing, we use a kind of NOP (otherwise
-           switch should handle option as a parameter, too many useless changes) *)
-        NOP
+        None
     end.
 
   Definition expr_of_trace (C: Component.id) (P: Procedure.id) (t: trace) : expr :=
-    switch (map (expr_of_event C P) (suffixes_of_seq t)) E_exit.
+    switch (pmap (expr_of_event C P) (suffixes_of_seq t)) E_exit.
 
   (** To compile a complete trace mixing events from different components, we
       split it into individual traces for each component and apply
@@ -969,11 +961,24 @@ Section Definability.
       | _ => false
       end.
   Hint Transparent filter_comp_subtrace.
+
   Definition comp_subtrace (C: Component.id) (t: trace) :=
     filter (filter_comp_subtrace C) t.
 
   Remark subseq_comp_subtrace C t : subseq (comp_subtrace C t) t.
   Proof. by apply filter_subseq. Qed.
+
+  Lemma length_comp_subtrace C P t : length (pmap (expr_of_event C P) (suffixes_of_seq (comp_subtrace C t))) =
+                                   length (filter (fun ev => ( C == cur_comp_of_event ev)) t).
+  Proof.
+    rewrite /comp_subtrace/filter_comp_subtrace. rewrite -!size_length size_pmap.
+    elim: t => //= ev t IHt.
+    case: ev => /= [????|??? |??? Cown] ; destruct (C == _) eqn:Ceq => //= ;
+        try (rewrite suffixes_of_seq_cons /= IHt -ssrnat.add1n ; apply/eqP ; rewrite ssrnat.eqn_add2r ;
+             case: (prefill_read _ _) => // ; by rewrite Ceq).
+    destruct (C == Cown) eqn:Ceq' ; last by rewrite IHt.
+    by rewrite suffixes_of_seq_cons /= IHt Ceq.
+  Qed.
 
   (* To relocate *)
   Lemma all_subseq {T:eqType} (s ss : seq T) (a : pred T) :
@@ -1110,6 +1115,8 @@ Section Definability.
       rewrite mkfmapfE; case: ifP=> //= P_CI [<-] {Pexpr}; split; last first.
       + (* values_are_integers *)
         rewrite /procedure_of_trace /expr_of_trace /switch.
+        (* Btw, would it be simpler to do induction by appending an event at the
+           end (with last_ind)? *)
         elim: {t Ht} (comp_subtrace C t) (length _) Hwf_sbt => [| e t IH] //= n /andP [_ Ht].
         have Hpref: forall expr, prefill_read C t = Some expr ->
                             values_are_integers expr
@@ -1121,7 +1128,6 @@ Section Definability.
           case: (prefill_read C t) Hpref => /= [ex|] Hpref ;
             try (apply/andP ; split ; first by (rewrite andbT ; apply Hpref)) ;
             try done.
-        all : apply /andP ; split ; last done.
         all : by case:(C==_).
       + (* Valid calls *)
         pose call_of_event e := if e is ECall _ P _ C then Some (C, P) else None.
@@ -1130,20 +1136,19 @@ Section Definability.
                   ((C, P) |: fset (pmap call_of_event (comp_subtrace C t))).
         { rewrite /procedure_of_trace /expr_of_trace /switch suffixes_of_seq_equiv.
           elim: {t Ht} (comp_subtrace C t) (length _) Hwf_sbt => [|e t IH] /= n Ht ;
-              first exact: fsub0set ; rewrite !fset0U.
+              first exact: fsub0set.
           move:Ht => /andP[_ Ht].
           have Hpref: forall expr, prefill_read C t = Some expr ->
                               called_procedures expr = fset0
               by move => ? ; apply (prefill_read_no_calls intf_C).
           specialize (IH n Ht).
           case: e => [C' P' arg C''| C' ret C'' | C' i v C''] ;
-                      last by (case: (C== _) => /= ; by rewrite !fset0U).
+                      last by (case: (C== _) => /= ; first rewrite !fset0U).
           all: case: (prefill_read C t) Hpref => [ex|] Hpref //= ;
                                                   first (rewrite (Hpref ex); last done);
-                                                  try by rewrite !fset0U.
-          rewrite fset0U.
-          all :rewrite !fsetU0 fset_cons !fsubUset !fsub1set !in_fsetU1 !eqxx !orbT /=.
-          all:by rewrite fsetUA [(C, P) |: _]fsetUC -fsetUA fsubsetU // IH orbT.
+                                                  rewrite !fset0U => //.
+          all: rewrite !fsetU0 fset_cons !fsubUset !fsub1set !in_fsetU1 !eqxx !orbT /=.
+          all: by rewrite fsetUA [(C, P) |: _]fsetUC -fsetUA fsubsetU // IH orbT.
         }
         (* Back to Valid calls *)
       move=> C' P' /sub/fsetU1P [[-> ->]|] {sub}.
@@ -1210,21 +1215,15 @@ Section Definability.
       by rewrite mem_domm; case=> ->.
     Qed.
 
-    (* So, either we change the definition to get what we had before (we filter
-       the ELoad events not triggered by the component out of the comp_subtrace)
-       or we take into account the ELoad events, *)
-    (* In the end, we just end up ruling out all ELoad events. But since this
-       affects the spec 'switch_spec_else', we won't change anything *)
+    (** equals to the number of events triggered by the component at this point
+     *)
     Local Definition counter_value C prefix :=
-      Z.of_nat (length (comp_subtrace C prefix)).
+      Z.of_nat (length (filter (fun ev => C == cur_comp_of_event ev) prefix)).
 
     Lemma counter_value_app C prefix1 prefix2 :
       counter_value C (prefix1 ++ prefix2)
       = (counter_value C prefix1 + counter_value C prefix2) % Z.
-    Proof.
-      unfold counter_value.
-      now rewrite comp_subtrace_app  app_length Nat2Z.inj_add.
-    Qed.
+    Proof. by rewrite /counter_value filter_cat app_length Nat2Z.inj_add. Qed.
 
     Definition well_formed_memory (prefix: trace) (mem: Memory.t) : Prop :=
       forall C,
@@ -1234,11 +1233,10 @@ Section Definability.
     Lemma counter_value_snoc prefix C e :
       counter_value C (prefix ++ [e])
       = (counter_value C prefix
-         + if (filter_comp_subtrace C) e
+         + if C == cur_comp_of_event e
            then 1 else 0) % Z.
     Proof.
       Print counter_value. rewrite /counter_value.
-      unfold counter_value, comp_subtrace, filter_comp_subtrace.
       rewrite filter_cat app_length. simpl.
       rewrite Nat2Z.inj_add.
       now destruct (_ == _) ; destruct e as [| |? ? ? C' ]=> //= ; case: (_ == _) => //.
@@ -1249,7 +1247,8 @@ Section Definability.
       well_formed_memory prefix mem ->
       C = cur_comp_of_event e ->
       exists mem',
-        Memory.store mem (C, Block.private, counter_idx) (Int (counter_value C (prefix ++ [e]))) = Some mem' /\
+        Memory.store mem (C, Block.private, counter_idx)
+                     (Int (counter_value C (prefix ++ [e]))) = Some mem' /\
         well_formed_memory (prefix ++ [e]) mem'.
     Proof.
       move=> C_b wf_mem HC.
@@ -1257,18 +1256,21 @@ Section Definability.
       have [mem' Hmem'] := Memory.store_after_load
                              _ _ _ (Int (counter_value C (prefix ++ [e])))
                              C_local.
-    (* RB: STATIC_READ: To fix. *)
-    (*   exists mem'. split; trivial=> C' C'_b. *)
-    (*   have C'_local := wf_mem _ C'_b. *)
-    (*   rewrite -> counter_value_snoc, <- HC, Nat.eqb_refl in *. *)
-    (*   case: (altP (C' =P C)) => [?|C_neq_C']. *)
-    (*   - subst C'. *)
-    (*     by rewrite -> (Memory.load_after_store_eq _ _ _ _ Hmem'). *)
-    (*   - have neq : (C, Block.local, counter_idx) <> (C', Block.local, counter_idx) by move/eqP in C_neq_C'; congruence. *)
-    (*     rewrite (Memory.load_after_store_neq _ _ _ _ _ neq Hmem'). *)
-    (*     now rewrite Z.add_0_r. *)
-    (* Qed. *)
-    Admitted.
+
+      exists mem'. split; trivial => C' C'_b.
+      have C'_local := wf_mem _ C'_b.
+      move:Hmem' ;
+        rewrite !counter_value_snoc -!HC => Hmem'.
+      rewrite -> Nat.eqb_refl in Hmem'.
+      case: (altP (C' =P C)) => [?|C_neq_C'].
+      - subst C'.
+        by rewrite -> (Memory.load_after_store_eq _ _ _ _ Hmem').
+      - have neq : (C, Block.private, counter_idx) <> (C', Block.private, counter_idx)
+          by move/eqP in C_neq_C'; congruence.
+        rewrite (Memory.load_after_store_neq _ _ _ _ _ neq Hmem').
+        case: e HC => [????|???|??? Cown] HC; last case:(C'==Cown) => // ;
+        rewrite Z.add_0_r ; assumption.
+    Qed.
 
     CoInductive well_formed_state (s: stack_state) (prefix suffix: trace) : CS.state -> Prop :=
     | WellFormedState C stk mem k exp arg P
@@ -1298,16 +1300,16 @@ Section Definability.
         have C_local := wf_mem _ C_b.
         rewrite /procedure_of_trace /expr_of_trace.
         apply: switch_spec_else; eauto.
-      (* RB: STATIC_READ: To fix. *)
-      (*   rewrite -> size_map; reflexivity. *)
-      (* - move=> cs Et /=. *)
-      (*   case: cs / => /= _ stk mem _ _ arg P -> -> -> /andP [/eqP wf_C wb_suffix] /andP [wf_e wf_suffix] wf_stk wf_mem P_exp. *)
-      (*   have C_b := valid_procedure_has_block P_exp. *)
-      (*   have C_local := wf_mem _ C_b. *)
-      (*   destruct (well_formed_memory_store_counter C_b wf_mem wf_C) as [mem' [Hmem' wf_mem']]. *)
+        by rewrite length_comp_subtrace.
+      - move=> cs Et /=.
+        case: cs / => /= _ stk mem _ _ arg P -> -> -> /andP [/eqP wf_C wb_suffix] /andP [wf_e wf_suffix] wf_stk wf_mem P_exp.
+        have C_b := valid_procedure_has_block P_exp.
+        have C_local := wf_mem _ C_b.
+        destruct (well_formed_memory_store_counter C_b wf_mem wf_C) as [mem' [Hmem' wf_mem']].
       (*   assert (Star1 : Star (CS.sem p) *)
       (*                        [CState C, stk, mem , Kstop, expr_of_trace C P (comp_subtrace C t), arg] E0 *)
-      (*                        [CState C, stk, mem', Kstop, expr_of_event C P e, arg]). *)
+      (*                        [CState C, stk, mem', Kstop, expr_of_event C P (e::suffix), arg]). *)
+
       (*   { unfold expr_of_trace. rewrite Et comp_subtrace_app. simpl. *)
       (*     rewrite <- wf_C, Nat.eqb_refl, map_app. simpl. *)
       (*     assert (H := @switch_spec p C  stk mem *)
